add nbe def

stlc/language.sig
@@ -10,6 +10,6 @@ typ_bool : typ
 exp_app   : exp -> exp -> exp
 -- no type annotations for arguments
 exp_abs   : (bind exp in exp) -> exp
-exp_if    : exp -> exp -> exp -> exp
+exp_if    : typ -> exp -> exp -> exp -> exp
 exp_true  : exp
 exp_false : exp
