stlc/def_as2.v
@@ -5,11 +5,27 @@ Require Import Setoid Morphisms Relation_Definitions.
 
 Module Core.
 
+Inductive typ : Type :=
+  | typ_arr : typ -> typ -> typ
+  | typ_bool : typ.
+
+Lemma congr_typ_arr {s0 : typ} {s1 : typ} {t0 : typ} {t1 : typ}
+  (H0 : s0 = t0) (H1 : s1 = t1) : typ_arr s0 s1 = typ_arr t0 t1.
+Proof.
+exact (eq_trans (eq_trans eq_refl (ap (fun x => typ_arr x s1) H0))
+         (ap (fun x => typ_arr t0 x) H1)).
+Qed.
+
+Lemma congr_typ_bool : typ_bool = typ_bool.
+Proof.
+exact (eq_refl).
+Qed.
+
 Inductive exp : Type :=
   | exp_var : nat -> exp
   | exp_app : exp -> exp -> exp
   | exp_abs : exp -> exp
-  | exp_if : exp -> exp -> exp -> exp
+  | exp_if : typ -> exp -> exp -> exp -> exp
   | exp_true : exp
   | exp_false : exp.
 
@@ -26,14 +42,16 @@ Proof.
 exact (eq_trans eq_refl (ap (fun x => exp_abs x) H0)).
 Qed.
 
-Lemma congr_exp_if {s0 : exp} {s1 : exp} {s2 : exp} {t0 : exp} {t1 : exp}
-  {t2 : exp} (H0 : s0 = t0) (H1 : s1 = t1) (H2 : s2 = t2) :
-  exp_if s0 s1 s2 = exp_if t0 t1 t2.
+Lemma congr_exp_if {s0 : typ} {s1 : exp} {s2 : exp} {s3 : exp} {t0 : typ}
+  {t1 : exp} {t2 : exp} {t3 : exp} (H0 : s0 = t0) (H1 : s1 = t1)
+  (H2 : s2 = t2) (H3 : s3 = t3) : exp_if s0 s1 s2 s3 = exp_if t0 t1 t2 t3.
 Proof.
 exact (eq_trans
-         (eq_trans (eq_trans eq_refl (ap (fun x => exp_if x s1 s2) H0))
-            (ap (fun x => exp_if t0 x s2) H1))
-         (ap (fun x => exp_if t0 t1 x) H2)).
+         (eq_trans
+            (eq_trans (eq_trans eq_refl (ap (fun x => exp_if x s1 s2 s3) H0))
+               (ap (fun x => exp_if t0 x s2 s3) H1))
+            (ap (fun x => exp_if t0 t1 x s3) H2))
+         (ap (fun x => exp_if t0 t1 t2 x) H3)).
 Qed.
 
 Lemma congr_exp_true : exp_true = exp_true.
@@ -56,8 +74,8 @@ Fixpoint ren_exp (xi_exp : nat -> nat) (s : exp) {struct s} : exp :=
   | exp_var s0 => exp_var (xi_exp s0)
   | exp_app s0 s1 => exp_app (ren_exp xi_exp s0) (ren_exp xi_exp s1)
   | exp_abs s0 => exp_abs (ren_exp (upRen_exp_exp xi_exp) s0)
-  | exp_if s0 s1 s2 =>
-      exp_if (ren_exp xi_exp s0) (ren_exp xi_exp s1) (ren_exp xi_exp s2)
+  | exp_if s0 s1 s2 s3 =>
+      exp_if s0 (ren_exp xi_exp s1) (ren_exp xi_exp s2) (ren_exp xi_exp s3)
   | exp_true => exp_true
   | exp_false => exp_false
   end.
@@ -73,9 +91,9 @@ Fixpoint subst_exp (sigma_exp : nat -> exp) (s : exp) {struct s} : exp :=
   | exp_app s0 s1 =>
       exp_app (subst_exp sigma_exp s0) (subst_exp sigma_exp s1)
   | exp_abs s0 => exp_abs (subst_exp (up_exp_exp sigma_exp) s0)
-  | exp_if s0 s1 s2 =>
-      exp_if (subst_exp sigma_exp s0) (subst_exp sigma_exp s1)
-        (subst_exp sigma_exp s2)
+  | exp_if s0 s1 s2 s3 =>
+      exp_if s0 (subst_exp sigma_exp s1) (subst_exp sigma_exp s2)
+        (subst_exp sigma_exp s3)
   | exp_true => exp_true
   | exp_false => exp_false
   end.
@@ -101,9 +119,9 @@ subst_exp sigma_exp s = s :=
   | exp_abs s0 =>
       congr_exp_abs
         (idSubst_exp (up_exp_exp sigma_exp) (upId_exp_exp _ Eq_exp) s0)
-  | exp_if s0 s1 s2 =>
-      congr_exp_if (idSubst_exp sigma_exp Eq_exp s0)
-        (idSubst_exp sigma_exp Eq_exp s1) (idSubst_exp sigma_exp Eq_exp s2)
+  | exp_if s0 s1 s2 s3 =>
+      congr_exp_if (eq_refl s0) (idSubst_exp sigma_exp Eq_exp s1)
+        (idSubst_exp sigma_exp Eq_exp s2) (idSubst_exp sigma_exp Eq_exp s3)
   | exp_true => congr_exp_true
   | exp_false => congr_exp_false
   end.
@@ -130,10 +148,10 @@ ren_exp xi_exp s = ren_exp zeta_exp s :=
       congr_exp_abs
         (extRen_exp (upRen_exp_exp xi_exp) (upRen_exp_exp zeta_exp)
            (upExtRen_exp_exp _ _ Eq_exp) s0)
-  | exp_if s0 s1 s2 =>
-      congr_exp_if (extRen_exp xi_exp zeta_exp Eq_exp s0)
-        (extRen_exp xi_exp zeta_exp Eq_exp s1)
+  | exp_if s0 s1 s2 s3 =>
+      congr_exp_if (eq_refl s0) (extRen_exp xi_exp zeta_exp Eq_exp s1)
         (extRen_exp xi_exp zeta_exp Eq_exp s2)
+        (extRen_exp xi_exp zeta_exp Eq_exp s3)
   | exp_true => congr_exp_true
   | exp_false => congr_exp_false
   end.
@@ -161,10 +179,10 @@ subst_exp sigma_exp s = subst_exp tau_exp s :=
       congr_exp_abs
         (ext_exp (up_exp_exp sigma_exp) (up_exp_exp tau_exp)
            (upExt_exp_exp _ _ Eq_exp) s0)
-  | exp_if s0 s1 s2 =>
-      congr_exp_if (ext_exp sigma_exp tau_exp Eq_exp s0)
-        (ext_exp sigma_exp tau_exp Eq_exp s1)
+  | exp_if s0 s1 s2 s3 =>
+      congr_exp_if (eq_refl s0) (ext_exp sigma_exp tau_exp Eq_exp s1)
         (ext_exp sigma_exp tau_exp Eq_exp s2)
+        (ext_exp sigma_exp tau_exp Eq_exp s3)
   | exp_true => congr_exp_true
   | exp_false => congr_exp_false
   end.
@@ -190,10 +208,11 @@ Fixpoint compRenRen_exp (xi_exp : nat -> nat) (zeta_exp : nat -> nat)
       congr_exp_abs
         (compRenRen_exp (upRen_exp_exp xi_exp) (upRen_exp_exp zeta_exp)
            (upRen_exp_exp rho_exp) (up_ren_ren _ _ _ Eq_exp) s0)
-  | exp_if s0 s1 s2 =>
-      congr_exp_if (compRenRen_exp xi_exp zeta_exp rho_exp Eq_exp s0)
+  | exp_if s0 s1 s2 s3 =>
+      congr_exp_if (eq_refl s0)
         (compRenRen_exp xi_exp zeta_exp rho_exp Eq_exp s1)
         (compRenRen_exp xi_exp zeta_exp rho_exp Eq_exp s2)
+        (compRenRen_exp xi_exp zeta_exp rho_exp Eq_exp s3)
   | exp_true => congr_exp_true
   | exp_false => congr_exp_false
   end.
@@ -223,10 +242,11 @@ Fixpoint compRenSubst_exp (xi_exp : nat -> nat) (tau_exp : nat -> exp)
       congr_exp_abs
         (compRenSubst_exp (upRen_exp_exp xi_exp) (up_exp_exp tau_exp)
            (up_exp_exp theta_exp) (up_ren_subst_exp_exp _ _ _ Eq_exp) s0)
-  | exp_if s0 s1 s2 =>
-      congr_exp_if (compRenSubst_exp xi_exp tau_exp theta_exp Eq_exp s0)
+  | exp_if s0 s1 s2 s3 =>
+      congr_exp_if (eq_refl s0)
         (compRenSubst_exp xi_exp tau_exp theta_exp Eq_exp s1)
         (compRenSubst_exp xi_exp tau_exp theta_exp Eq_exp s2)
+        (compRenSubst_exp xi_exp tau_exp theta_exp Eq_exp s3)
   | exp_true => congr_exp_true
   | exp_false => congr_exp_false
   end.
@@ -267,10 +287,11 @@ ren_exp zeta_exp (subst_exp sigma_exp s) = subst_exp theta_exp s :=
       congr_exp_abs
         (compSubstRen_exp (up_exp_exp sigma_exp) (upRen_exp_exp zeta_exp)
            (up_exp_exp theta_exp) (up_subst_ren_exp_exp _ _ _ Eq_exp) s0)
-  | exp_if s0 s1 s2 =>
-      congr_exp_if (compSubstRen_exp sigma_exp zeta_exp theta_exp Eq_exp s0)
+  | exp_if s0 s1 s2 s3 =>
+      congr_exp_if (eq_refl s0)
         (compSubstRen_exp sigma_exp zeta_exp theta_exp Eq_exp s1)
         (compSubstRen_exp sigma_exp zeta_exp theta_exp Eq_exp s2)
+        (compSubstRen_exp sigma_exp zeta_exp theta_exp Eq_exp s3)
   | exp_true => congr_exp_true
   | exp_false => congr_exp_false
   end.
@@ -313,10 +334,11 @@ subst_exp tau_exp (subst_exp sigma_exp s) = subst_exp theta_exp s :=
       congr_exp_abs
         (compSubstSubst_exp (up_exp_exp sigma_exp) (up_exp_exp tau_exp)
            (up_exp_exp theta_exp) (up_subst_subst_exp_exp _ _ _ Eq_exp) s0)
-  | exp_if s0 s1 s2 =>
-      congr_exp_if (compSubstSubst_exp sigma_exp tau_exp theta_exp Eq_exp s0)
+  | exp_if s0 s1 s2 s3 =>
+      congr_exp_if (eq_refl s0)
         (compSubstSubst_exp sigma_exp tau_exp theta_exp Eq_exp s1)
         (compSubstSubst_exp sigma_exp tau_exp theta_exp Eq_exp s2)
+        (compSubstSubst_exp sigma_exp tau_exp theta_exp Eq_exp s3)
   | exp_true => congr_exp_true
   | exp_false => congr_exp_false
   end.
@@ -402,10 +424,10 @@ Fixpoint rinst_inst_exp (xi_exp : nat -> nat) (sigma_exp : nat -> exp)
       congr_exp_abs
         (rinst_inst_exp (upRen_exp_exp xi_exp) (up_exp_exp sigma_exp)
            (rinstInst_up_exp_exp _ _ Eq_exp) s0)
-  | exp_if s0 s1 s2 =>
-      congr_exp_if (rinst_inst_exp xi_exp sigma_exp Eq_exp s0)
-        (rinst_inst_exp xi_exp sigma_exp Eq_exp s1)
+  | exp_if s0 s1 s2 s3 =>
+      congr_exp_if (eq_refl s0) (rinst_inst_exp xi_exp sigma_exp Eq_exp s1)
         (rinst_inst_exp xi_exp sigma_exp Eq_exp s2)
+        (rinst_inst_exp xi_exp sigma_exp Eq_exp s3)
   | exp_true => congr_exp_true
   | exp_false => congr_exp_false
   end.
@@ -468,22 +490,6 @@ Lemma varLRen'_exp_pointwise (xi_exp : nat -> nat) :
     (funcomp (exp_var) xi_exp).
 Proof.
 exact (fun x => eq_refl).
-Qed.
-
-Inductive typ : Type :=
-  | typ_arr : typ -> typ -> typ
-  | typ_bool : typ.
-
-Lemma congr_typ_arr {s0 : typ} {s1 : typ} {t0 : typ} {t1 : typ}
-  (H0 : s0 = t0) (H1 : s1 = t1) : typ_arr s0 s1 = typ_arr t0 t1.
-Proof.
-exact (eq_trans (eq_trans eq_refl (ap (fun x => typ_arr x s1) H0))
-         (ap (fun x => typ_arr t0 x) H1)).
-Qed.
-
-Lemma congr_typ_bool : typ_bool = typ_bool.
-Proof.
-exact (eq_refl).
 Qed.
 
 Class Up_exp X Y :=
