stlc/def_nbe.v
@@ -1,0 +1,113 @@
+Require Import Coq.Program.Equality.
+
+Require Import nbe.stlc.def_as2.
+Require Import nbe.stlc.def_syntax.
+
+Inductive d : Set :=
+  | d_true
+  | d_false
+  | d_abs (t : exp) (ρ : nat -> d)
+  | d_refl (T: typ) (e : d_ne)
+with d_ne : Set :=
+  | dne_l (n : nat) 
+  | dne_if (T : typ) (e : d_ne) (dt df : d_nf)
+  | dne_app (e : d_ne) (d : d_nf)
+with d_nf : Set :=
+  | dnf_reif (T : typ) (a : d).
+
+Notation " ( 'ƛ' t ) ρ " := (d_abs t ρ)
+  (at level 55).
+
+Definition env := nat -> d.
+
+Definition add (ρ : env) (d : d) : env :=
+  fun n => match n with 
+    | 0 => d
+    | S n => ρ n
+    end.
+
+Definition drop : env -> env :=
+  fun ρ n => ρ (S n).
+
+Notation "ρ ↦ d" := (add ρ d)
+  (at level 48, left associativity).
+
+Reserved Notation "f ∙ a ↘ b"
+  (at level 55, a at next level, no associativity).
+Reserved Notation "⟦ t ⟧ ρ ↘ a"
+  (at level 55, ρ at next level, no associativity).
+Reserved Notation "if( T , db , dt , df ) ↘ d"
+  (at level 55, db at next level, dt at next level, df at next level, no associativity).
+Inductive eval_rel : exp -> env -> d -> Prop :=
+  | eval_true : forall ρ,
+    ⟦ exp_true ⟧ ρ ↘ d_true
+  | eval_false : forall ρ,
+    ⟦ exp_false ⟧ ρ ↘ d_false
+  | eval_var : forall ρ n,
+    ⟦ exp_var n ⟧ ρ ↘ (ρ n)
+  | eval_abs : forall ρ t,
+    ⟦ exp_abs t ⟧ ρ ↘ (d_abs t ρ)
+  | eval_app : forall ρ r s f a b,
+    ⟦ r ⟧ ρ ↘ f ->
+    ⟦ s ⟧ ρ ↘ a ->
+    f ∙ a ↘ b ->
+    ⟦ exp_app r s ⟧ ρ ↘ b
+with app_rel : d -> d -> d -> Prop :=
+  | app_abs : forall t ρ a b,
+    ⟦ t ⟧ (ρ ↦ a) ↘ b ->
+    (d_abs t ρ) ∙ a ↘ b
+  | app_app : forall e d S T,
+    (d_refl (S → T) e) ∙ d ↘ (d_refl T (dne_app e ( dnf_reif S d )))
+with if_rel : typ -> d -> d -> d -> d -> Prop :=
+  | if_true : forall dt df T,
+    if( T , d_true , dt , df ) ↘ dt
+  | if_false : forall dt df T,
+    if( T , d_false , dt , df ) ↘ df
+  | rec_rec : forall dt df e T,
+    if( T , d_refl typ_bool e , dt , df) ↘ d_refl T (dne_if T e (dnf_reif T dt) (dnf_reif T df))
+where "f ∙ a ↘ b" := (app_rel f a b) and 
+      "⟦ t ⟧ ρ ↘ a" := (eval_rel t ρ a) and 
+      "if( T , db , dt , df ) ↘ d" := (if_rel T db dt df d).
+
+Reserved Notation " 'Rⁿᶠ' ⦇ n ⦈ d ↘ v"
+  (at level 55, d at next level, no associativity).
+Reserved Notation " 'Rⁿᵉ' ⦇ n ⦈ e ↘ u"
+  (at level 55, e at next level, no associativity).
+Inductive rnf_rel : nat -> d_nf -> nf -> Prop := 
+  | rnf_abs : forall f b n t S T,
+    f ∙ (d_refl S (dne_l n)) ↘ b ->
+    Rⁿᶠ ⦇ 1 + n ⦈ (dnf_reif T b) ↘ t ->
+    Rⁿᶠ ⦇ n ⦈ (dnf_reif (S → T) f) ↘ (nf_abs t)
+  | rnf_true : forall n,
+    Rⁿᶠ ⦇ n ⦈ (dnf_reif typ_bool d_true) ↘ nf_true
+  | rnf_false : forall n,
+    Rⁿᶠ ⦇ n ⦈ (dnf_reif typ_bool d_false) ↘ nf_false
+  | rnf_ne : forall n e t,
+    Rⁿᵉ ⦇ n ⦈ e ↘ t ->
+    Rⁿᶠ ⦇ n ⦈ (dnf_reif typ_bool (d_refl typ_bool e)) ↘ (nf_ne t)
+with rne_rel : nat -> d_ne -> ne -> Prop :=
+  | rne_v : forall n k,
+    Rⁿᵉ ⦇ n ⦈ (dne_l k) ↘ (ne_v (n - k - 1))
+  | rne_app : forall n e d u v,
+    Rⁿᵉ ⦇ n ⦈ e ↘ u ->
+    Rⁿᶠ ⦇ n ⦈ d ↘ v ->
+    Rⁿᵉ ⦇ n ⦈ (dne_app e d) ↘ (ne_app u v)
+  | rne_if : forall n e dt df u vt vf T,
+    Rⁿᵉ ⦇ n ⦈ e ↘ u ->
+    Rⁿᶠ ⦇ n ⦈ dt ↘ vt ->
+    Rⁿᶠ ⦇ n ⦈ df ↘ vf ->
+    Rⁿᵉ ⦇ n ⦈ (dne_if T e dt df) ↘ (ne_if T u vt vf)
+where " 'Rⁿᶠ' ⦇ n ⦈ d ↘ v" := (rnf_rel n d v) and 
+      " 'Rⁿᵉ' ⦇ n ⦈ e ↘ u" := (rne_rel n e u).
+
+Definition Nbe (n : nat) (ρ : env) (t : exp) (T: typ) (w : nf) :=
+  exists a, ⟦ t ⟧ ρ ↘ a /\ Rⁿᶠ ⦇ n ⦈ (dnf_reif T a) ↘ w.
+
+Definition Completenss' (n : nat) (ρ ρ' : env) (s t : exp) (T : typ) :=
+  exists w, Nbe n ρ s T w /\ Nbe n ρ' t T w.
+
+Definition Completenss (n : nat) (ρ : env) (s t : exp) (T : typ) :=
+  exists w, Nbe n ρ s T w /\ Nbe n ρ t T w.
+
+Definition Soundness (Γ : ctx) (t : exp) (T : typ) (ρ : env) : Prop :=
+  exists w, Nbe (length Γ) ρ t T w /\ Γ ⊢ t ≈ w : T.
